## 引理$\textbf{1}$的内容

👉前提：$X\sim{}N(0,\sigma)$即$f(x)\text{=}\cfrac{1}{\sqrt{2\pi}\sigma}e^{–\frac{x^{2}}{2\sigma^{2}}}$，且$\forall{}\alpha{}\text{<}\cfrac{1}{2\sigma^{2}}$

👉结论：$\mathbb{E}\left[e^{\alpha{}X^{2}}\right]\text{=}\cfrac{1}{\sqrt{1–2\alpha{}\sigma^{2}}}$

## 结论的证明​​

➡️$\displaystyle{}\mathbb{E}\left[e^{\alpha{}X^2}\right]\text{=}\int_{–\infty}^{\infty}e^{\alpha{}x^2}f(x)dx\text{=}\int_{–\infty}^{\infty}e^{\alpha{}x^2}\frac{1}{\sqrt{2\pi}\sigma}e^{–\frac{x^2}{2\sigma^2}}dx\text{=}\int_{–\infty}^{\infty}\frac{1}{\sqrt{2\pi}\sigma}e^{–\frac{x^2}{2\sigma^2}\left(1–2\alpha\sigma^2\right)}dx$

➡️令$\sigma^{\prime}=\cfrac{\sigma}{\sqrt{1–2\alpha\sigma^2}}$，其中必定要求$1–2\alpha\sigma^2\text{>0}$即$\alpha{}\text{<}\cfrac{1}{2\sigma^{2}}$

➡️$\displaystyle{}\mathbb{E}\left[e^{\alpha{}X^2}\right]\text{=}\int_{–\infty}^{\infty}\cfrac{\sqrt{1–2\alpha\sigma^2}}{\sqrt{2\pi}\sigma\sqrt{1–2\alpha\sigma^2}}e^{–\frac{x^2}{2\sigma^2}\left(1–2\alpha\sigma^2\right)}dx\text{=}\cfrac{1}{\sqrt{1–2\alpha{}\sigma^{2}}}\int_{-\infty}^{\infty}\cfrac{1}{\sqrt{2\pi}\sigma^{\prime}}e^{-\frac{x^2}{2\sigma^{\prime2}}}dx$

➡️考虑到$\displaystyle{}\int_{-\infty}^{\infty}\frac{1}{\sqrt{2\pi}\sigma^{\prime}}e^{-\frac{x^2}{2\sigma^{\prime2}}}dx\text{=}1$，所以$\mathbb{E}\left[e^{\alpha{}X^{2}}\right]\text{=}\cfrac{1}{\sqrt{1–2\alpha{}\sigma^{2}}}$

